Use set to keep track of all the allocated keys

theories/case_studies/multiuser_kvs/kvs_preamble.v
@@ -13,6 +13,33 @@ Class kvsG Σ :=
       kvs_genG :: gen_heapGS nat kvs_entry Σ;
     }.
 
+
+Definition allocated_keys_auth `{kvsG} ( s : gset (Z * Z) ) : iProp Σ. Admitted.
+Definition allocated_keys_frag `{kvsG} (ku : Z) ( s : gset (Z*Z) ) : iProp Σ. Admitted.
+
+Notation "●(ALLOC) s" := (allocated_keys_auth s)%I (at level 20) : bi_scope.
+Notation "◯(ALLOC)[ k ] s" := (allocated_keys_frag k s)%I (at level 20) : bi_scope.
+
+Lemma allocated_keys_valid `{kvsG} (ku : Z) (s s' : gset (Z * Z)) :
+  ●(ALLOC) s -∗ ◯(ALLOC)[ ku ] s' -∗ ⌜ s' = filter (λ k, k.1 = ku) s ⌝.
+Proof.
+Admitted.
+
+Lemma allocated_keys_union `{kvsG} (ku : Z) (s s' s'' : gset (Z * Z)) :
+  (forall k, k ∈ s'' -> k.1 = ku) ->
+  ●(ALLOC) s -∗ ◯(ALLOC)[ku] s' ==∗ ●(ALLOC) (s'' ∪ s) ∗ ◯(ALLOC)[ku] (s'' ∪ s').
+Proof.
+Admitted.
+
+Lemma allocated_keys_insert `{kvsG} (ku : Z)  (kn : Z) (s s' : gset (Z * Z)) :
+  ●(ALLOC) s -∗ ◯(ALLOC)[ku] s' ==∗
+  ●(ALLOC) ( {[ (ku, kn) ]} ∪ s) ∗ ◯(ALLOC)[ku] ( {[ (ku, kn) ]} ∪ s').
+Proof.
+  iIntros "Hs Hs'".
+  iMod (allocated_keys_union with "Hs Hs'") as "[$ $]" ; last done.
+  intros k Hk. apply elem_of_singleton in Hk ; simplify_eq; done.
+Qed.
+
 Definition kvs_frag_idx_frac `{kvsG} (idx : nat) (k : Z) (w : Word) (q : dfrac) : iProp Σ :=
   (pointsto (L:=nat) (V:=kvs_entry) idx q (k,w)).
 Notation "k '⤇(KVS){' q '}[' idx  ']' w" :=
@@ -31,44 +58,6 @@ Notation "k '⤇(KVS)' -" := (∃ w, kvs_frag k w)%I (at level 20) : bi_scope.
 
 Notation "●(KVS) m" := (gen_heap_interp (m : kvs_map)) (at level 20) : bi_scope.
 
-(* TODO move + surely there's a better way to prove this *)
-Lemma NoDup_map_to_list_snd_fst_insert {Key : Type} {Val1 Val2 : Type}
-  `{EqDecision Key} `{Countable Key}
-  (m : gmap Key (Val1 * Val2)) (k : Key) (kv : Val1) (vv1 vv2 : Val2) :
-  m !! k = Some (kv, vv1) ->
-  NoDup (map_to_list m).*2.*1 ->
-  NoDup (map_to_list (<[k := (kv, vv2)]>m)).*2.*1.
-Proof.
-  generalize dependent k; generalize dependent vv1.
-  induction m using map_ind; intros vv1 k Hk Hnodup; first simplify_map_eq.
-  destruct (decide (k = i)); simplify_map_eq.
-  - rewrite insert_insert_eq.
-    rewrite map_to_list_insert; auto.
-    rewrite map_to_list_insert in Hnodup; auto.
-  - rewrite insert_insert_ne; last done.
-    rewrite map_to_list_insert in Hnodup; last done.
-    rewrite map_to_list_insert; last by simplify_map_eq.
-    destruct x as [kX vX]; cbn in *.
-    apply NoDup_cons in Hnodup as [HkX Hnodup].
-    apply NoDup_cons; split.
-    + intro; apply HkX.
-      rewrite list_elem_of_fmap in H1; destruct H1 as ( [? ?] & ? & H1 ); simplify_eq.
-      rewrite list_elem_of_fmap in H1; destruct H1 as ( [? [? ?] ] & ? & H1 ); cbn in *; simplify_eq.
-      apply elem_of_map_to_list in H1.
-      destruct (decide (k = k0)); simplify_map_eq.
-      * rewrite list_elem_of_fmap.
-        exists (v1, vv1); split; first done.
-        rewrite list_elem_of_fmap.
-        exists (k0, (v1, vv1)); split; first done.
-        by apply elem_of_map_to_list.
-      * rewrite list_elem_of_fmap.
-        exists (v1, v2); split; first done.
-        rewrite list_elem_of_fmap.
-        exists (k0, (v1, v2)); split; first done.
-        by apply elem_of_map_to_list.
-    + eapply IHm; eauto.
-Qed.
-
 Section KVS_preamble.
   Context
     {Σ:gFunctors}
@@ -80,30 +69,41 @@ Section KVS_preamble.
     {swlayout : switcherLayout}
   .
 
-  Definition wf_kvs_map (m : kvs_map) : Prop :=
-    dom m = kvs_dom ∧ NoDup (fst <$> (snd <$> (map_to_list m))).
+  Definition kvs_keys (m : kvs_map) : list Z :=
+    (* filter (fun k -> k ≠ EMPTY_SLOT) (map_to_list m).*2.*1. *)
+    (map_to_list m).*2.*1.
 
-  Definition isKVS_entry_empty (idx : nat) (k : Z) (w : Word) : iProp Σ :=
-    (if (decide (k = EMPTY_SLOT)) then k ⤇(KVS)[idx] w else True)%I.
+  Definition wf_kvs_map (m : kvs_map) : Prop :=
+    dom m = kvs_dom ∧ NoDup (kvs_keys m).
+
+  Definition isKVS_entry_empty (idx : nat) (k : Z) : iProp Σ :=
+    (if (decide (k = EMPTY_SLOT)) then EMPTY_SLOT ⤇(KVS)[idx] (WInt DEFAULT_VAL) else True)%I.
 
   Definition isKVS_entry (a : Addr) (idx : nat) (kw : Z * Word) : iProp Σ :=
     let k := kw.1 in
     let w := kw.2 in
     (a ^+ (2*idx))%a ↦ₐ (WInt k) ∗
     (a ^+ (2*idx + 1))%a ↦ₐ w ∗
-    isKVS_entry_empty idx k w
+    isKVS_entry_empty idx k
   .
 
+  Definition kvs_alloc_synced (m : kvs_map) (s : gset (Z * Z)) : Prop :=
+    ∀ k, k ∈ s ↔ (kvs_full_key k.1 k.2) ∈ kvs_keys m.
+
   Definition isKVS
-    (a : Addr) (m : kvs_map) : iProp Σ :=
+    (a : Addr) (m : kvs_map) (s : gset (Z * Z)) : iProp Σ :=
     ⌜ wf_kvs_map m ⌝ ∗
     ●(KVS) m ∗
+    ●(ALLOC) s ∗
+    ⌜ kvs_alloc_synced m s ⌝ ∗
     [∗ map] idx ↦ kw ∈ m, isKVS_entry a idx kw.
 
   Definition isKVS_open
-    (a : Addr) (m : kvs_map) (open_idx : nat) : iProp Σ :=
+    (a : Addr) (m : kvs_map) (s : gset (Z * Z)) (open_idx : nat) : iProp Σ :=
     ⌜ wf_kvs_map m ⌝ ∗
     ●(KVS) m ∗
+    ●(ALLOC) s ∗
+    ⌜ kvs_alloc_synced m s ⌝ ∗
     [∗ map] idx ↦ kw ∈ (delete open_idx m), isKVS_entry a idx kw.
 
   Lemma wf_kvs_is_Some (m : kvs_map) (idx : nat)  :
@@ -136,6 +136,7 @@ Section KVS_preamble.
     k ≠ k'.
   Proof.
     intros [_ Hkvs_uniqueness] Hidx_ne Hm_idx Hm_idx'.
+    rewrite /kvs_keys in Hkvs_uniqueness.
     rewrite -(insert_id m idx (k, w)) in Hkvs_uniqueness; last done.
     rewrite -insert_delete_eq in Hkvs_uniqueness.
     rewrite -(insert_id (<[idx:=(k, w)]> (delete idx m)) idx' (k', w')) in Hkvs_uniqueness; last by simplify_map_eq.
@@ -148,7 +149,145 @@ Section KVS_preamble.
     set_solver+Hkvs_uniqueness.
   Qed.
 
+  Lemma elem_of_kvs_keys_1 (m : kvs_map) (k : Z) :
+    k ∈ kvs_keys m -> ∃ idx w, m !! idx = Some (k, w).
+  Proof.
+    intros Hk.
+    apply list_elem_of_fmap in Hk as ([k' v'] & ? & Hk); cbn in *; simplify_eq.
+    apply list_elem_of_fmap in Hk as ([idx' kv'] & ? & Hk); cbn in *; simplify_eq.
+    apply elem_of_map_to_list in Hk.
+    eauto.
+  Qed.
+
+  Lemma elem_of_kvs_keys_2 (m : kvs_map) (k : Z) :
+    (∃ idx w, m !! idx = Some (k, w)) -> k ∈ kvs_keys m.
+  Proof.
+    intros (idx & w & Hidx).
+    apply list_elem_of_fmap; exists (k, w); split; first done.
+    apply list_elem_of_fmap; exists (idx, (k, w)); split; first done.
+    by apply elem_of_map_to_list.
+  Qed.
+
+  Lemma elem_of_kvs_keys (m : kvs_map) (k : Z) :
+    k ∈ kvs_keys m ↔ ∃ idx w, m !! idx = Some (k, w).
+  Proof. split ; [apply elem_of_kvs_keys_1 | apply elem_of_kvs_keys_2]. Qed.
+
+
+  Lemma NoDup_kvs_keys_update (m : kvs_map) (idx : nat) (k : Z) (w w' : Word) :
+    m !! idx = Some (k, w) ->
+    NoDup (kvs_keys m) ->
+    NoDup (kvs_keys (<[idx := (k, w')]>m)).
+  Proof.
+    generalize dependent idx; generalize dependent w.
+    rewrite /kvs_keys.
+    induction m using map_ind; intros w idx Hk Hnodup; first simplify_map_eq.
+    destruct (decide (idx = i)); simplify_map_eq.
+    - rewrite insert_insert_eq.
+      rewrite map_to_list_insert; auto.
+      rewrite map_to_list_insert in Hnodup; auto.
+    - rewrite insert_insert_ne; last done.
+      rewrite map_to_list_insert in Hnodup; last done.
+      rewrite map_to_list_insert; last by simplify_map_eq.
+      destruct x as [kX vX]; cbn in *.
+      apply NoDup_cons in Hnodup as [HkX Hnodup].
+      apply NoDup_cons; split.
+      + rewrite -/(kvs_keys (<[idx:=(k, w')]> m)).
+        rewrite -/(kvs_keys m) in HkX.
+        intro Hcontra; apply HkX.
+        apply elem_of_kvs_keys in Hcontra as (idx0 & w0 & H0).
+        apply elem_of_kvs_keys.
+        destruct (decide (idx = idx0)); simplify_map_eq; eauto.
+      + eapply IHm; eauto.
+  Qed.
+
+  Lemma NoDup_kvs_keys_insert
+    (m : kvs_map) (idx : nat) (k : Z) (w : Word) :
+    k ∉ kvs_keys m ->
+    NoDup (kvs_keys m) ->
+    NoDup (kvs_keys (<[idx:=(k, w)]> m)).
+  Proof.
+    generalize dependent k.
+    generalize dependent w.
+    rewrite /kvs_keys.
+    induction m using map_ind; intros w k Hk Hnodup; first simplify_map_eq.
+    { rewrite map_to_list_insert; auto; cbn.
+      rewrite map_to_list_empty; auto; cbn.
+      apply NoDup_singleton.
+    }
+    destruct (decide (idx = i)); simplify_map_eq.
+    - rewrite insert_insert_eq.
+      rewrite map_to_list_insert; auto; cbn.
+      rewrite map_to_list_insert in Hnodup; auto; cbn in Hnodup.
+      rewrite map_to_list_insert in Hk; auto; cbn in Hk.
+      apply NoDup_cons in Hnodup as [_ Hnodup].
+      apply not_elem_of_cons in Hk as [_ Hk].
+      apply NoDup_cons; split; auto.
+    - rewrite insert_insert_ne; last done.
+      rewrite map_to_list_insert in Hnodup; last done.
+      rewrite map_to_list_insert in Hk; last done.
+      rewrite map_to_list_insert; last by simplify_map_eq.
+      destruct x as [kX vX]; cbn in *.
+      apply not_elem_of_cons in Hk as [Hk_ne Hk].
+      apply NoDup_cons in Hnodup as [HkX Hnodup].
+      apply NoDup_cons; split.
+      + rewrite -/(kvs_keys (<[idx:=(k, w)]> m)).
+        rewrite -/(kvs_keys m) in HkX.
+        intro Hcontra; apply HkX.
+        apply elem_of_kvs_keys in Hcontra as (idx0 & w0 & H0).
+        apply elem_of_kvs_keys.
+        destruct (decide (idx = idx0)); simplify_map_eq; eauto.
+      + eapply IHm; eauto.
+  Qed.
+
   Lemma wf_kvs_map_insert (m : kvs_map) (idx : nat) (k : Z) (w : Word) :
+    m !! idx = Some (EMPTY_SLOT, WInt DEFAULT_VAL) ->
+    k ∉ kvs_keys m ->
+    wf_kvs_map m ->
+    wf_kvs_map (<[idx:=(k, w)]> m).
+  Proof.
+    intros Hidx Hk (Hkvs_dom & Hkvs_unique).
+    split.
+    - rewrite dom_insert_L -Hkvs_dom.
+      assert (idx ∈ dom m).
+      { apply elem_of_dom; eauto. }
+      set_solver.
+    - eapply NoDup_kvs_keys_insert; eauto.
+  Qed.
+
+  Lemma kvs_alloc_synced_insert (m : kvs_map) ( s : gset (Z*Z) ) (idx : nat) (ku kn : Z) (w : Word) :
+    let fkey := kvs_full_key ku kn in
+    m !! idx = Some (EMPTY_SLOT, WInt DEFAULT_VAL) ->
+    fkey ∉ kvs_keys m ->
+    kvs_alloc_synced m s ->
+    kvs_alloc_synced (<[idx:=(fkey, w)]> m) ( {[ (ku, kn) ]} ∪ s).
+  Proof.
+    intros fkey Hidx Hk_free Halloc.
+    rewrite /kvs_alloc_synced.
+    intros [ku' kn'].
+    cbn.
+    specialize (Halloc (ku', kn')); cbn in *.
+    split; intros Hk.
+    - apply elem_of_union in Hk; destruct Hk as [Hk | Hk].
+      + apply elem_of_singleton in Hk ; simplify_eq.
+        eapply elem_of_kvs_keys.
+        by exists idx, w; simplify_map_eq.
+      + apply Halloc in Hk.
+        apply elem_of_kvs_keys in Hk as (idx' & v' & Hk).
+        eapply elem_of_kvs_keys.
+        destruct (decide (idx = idx')); simplify_map_eq; cbn in *; auto.
+        * admit. (* see kvs_full_key_not_empty *)
+        * by eexists idx', v'; simplify_map_eq.
+    - apply elem_of_union.
+      apply elem_of_kvs_keys in Hk as (idx' & v' & Hk).
+      destruct (decide (idx = idx')); simplify_map_eq; cbn in *; auto.
+      + left. apply elem_of_singleton.
+        (* see kvs_full_key_inj *)
+      + right.
+        apply Halloc.
+        by eapply elem_of_kvs_keys; eexists idx',_; simplify_map_eq.
+  Admitted.
+
+  Lemma wf_kvs_map_update (m : kvs_map) (idx : nat) (k : Z) (w : Word) :
     (∃ w', m !! idx = Some (k, w')) ->
     wf_kvs_map m ->
     wf_kvs_map (<[idx:=(k, w)]> m).
@@ -159,7 +298,7 @@ Section KVS_preamble.
       assert (idx ∈ dom m).
       { apply elem_of_dom; eauto. }
       set_solver.
-    - eapply NoDup_map_to_list_snd_fst_insert; eauto.
+    - eapply NoDup_kvs_keys_update; eauto.
   Qed.
 
   Lemma kvs_frag_kvs_frag_idx (k : Z) (w : Word) :
@@ -187,9 +326,9 @@ Section KVS_preamble.
     destruct H; eapply dfrac_full_exclusive in H; auto.
   Qed.
 
-  Lemma kvs_frag_kvs_empty_not_empty_slot idx k w w' :
+  Lemma kvs_frag_kvs_empty_not_empty_slot idx k w :
     k ⤇(KVS)[ idx ] w -∗
-    isKVS_entry_empty idx k w' -∗
+    isKVS_entry_empty idx k -∗
     ⌜ k ≠ EMPTY_SLOT ⌝.
   Proof.
     iIntros "Hk Hk'".
@@ -207,104 +346,207 @@ Section KVS_preamble.
     by iDestruct (gen_heap_valid with "Hkvs_auth Hk") as "%Hidx'".
   Qed.
 
-  Lemma isKVS_valid (m : kvs_map) (a : Addr) (idx : nat) (k : Z) (w : Word) :
-    isKVS a m -∗
+  Lemma isKVS_valid (m : kvs_map) (s : gset (Z*Z)) (a : Addr) (idx : nat) (k : Z) (w : Word) :
+    isKVS a m s -∗
     k ⤇(KVS)[idx] w -∗
     ⌜ m !! idx = Some (k, w) ⌝.
   Proof.
-    iIntros "(%HdomKVS & Hkvs_auth & HKVS) Hk".
+    iIntros "(%Hwf_kvs & Hkvs_auth & _) Hk".
     by iDestruct (kvs_valid with "Hkvs_auth Hk") as "%Hidx'".
   Qed.
 
-  Lemma isKVS_open_valid (m : kvs_map) (a : Addr) (idx idx' : nat) (k : Z) (w : Word) :
-    isKVS_open a m idx' -∗
+  Lemma isKVS_open_valid (m : kvs_map) (s : gset (Z*Z)) (a : Addr) (idx idx' : nat) (k : Z) (w : Word) :
+    isKVS_open a m s idx' -∗
     k ⤇(KVS)[idx] w -∗
     ⌜ m !! idx = Some (k, w) ⌝.
   Proof.
-    iIntros "(%HdomKVS & Hkvs_auth & HKVS) Hk".
+    iIntros "(%Hwf_kvs & Hkvs_auth & _) Hk".
     by iDestruct (kvs_valid with "Hkvs_auth Hk") as "%Hidx'".
   Qed.
 
   Lemma open_isKVS_kvs_frag_idx
-    (b : Addr) (m : kvs_map)
+    (b : Addr) (m : kvs_map) (s : gset (Z*Z))
     (idx : nat) (k : Z) (w : Word) :
-    isKVS b m ∗
+    isKVS b m s ∗
     k ⤇(KVS)[idx] w -∗
-    isKVS_open b m idx ∗
+    isKVS_open b m s idx ∗
     isKVS_entry b idx (k, w) ∗
     k ⤇(KVS)[idx] w.
   Proof.
-    iIntros "( (%HdomKVS & Hkvs_auth & HKVS) & Hk)".
+    iIntros "( (%Hwf_kvs & Hkvs_auth & Halloc & %Hwf_alloc & HKVS) & Hk)".
     iDestruct (gen_heap_valid with "Hkvs_auth Hk") as "%Hidx'".
     rewrite -{2}(insert_id m idx (k,w)); last done.
     iDestruct (big_sepM_insert_delete with "HKVS") as "[Hkvs_entry HKVS]".
     iFrame; eauto.
   Qed.
 
-  Lemma isKVS_indom_idx (m : kvs_map) (a : Addr) (idx : nat) :
+  Lemma isKVS_indom_idx (m : kvs_map) (s : gset (Z*Z)) (a : Addr) (idx : nat) :
     idx ∈ dom m ->
-    isKVS a m -∗
+    isKVS a m s -∗
     ⌜ 0 <= idx < SIZE_MAP ⌝.
   Proof.
-    iIntros (Hm_idx) "(%Hwf & _)"; iPureIntro.
+    iIntros (Hm_idx) "(%Hwf_kvs & _)"; iPureIntro.
     by eapply wf_kvs_indom_idx.
   Qed.
 
-  Lemma isKVS_open_indom_idx (m : kvs_map) (a : Addr) (idx idx' : nat) :
+  Lemma isKVS_open_indom_idx (m : kvs_map) (s : gset (Z*Z)) (a : Addr) (idx idx' : nat) :
     idx ∈ dom m ->
-    isKVS_open a m idx' -∗
+    isKVS_open a m s idx' -∗
     ⌜ 0 <= idx < SIZE_MAP ⌝.
   Proof.
-    iIntros (Hm_idx) "(%Hwf & _)"; iPureIntro.
+    iIntros (Hm_idx) "(%Hwf_kvs & _)"; iPureIntro.
     by eapply wf_kvs_indom_idx.
   Qed.
 
   Lemma open_isKVS_kvs_frag_idx_diff
-    (b : Addr) (m : kvs_map) (idx idx' : nat) (k : Z) (w : Word):
+    (b : Addr) (m : kvs_map) (s : gset (Z*Z)) (idx idx' : nat) (k : Z) (w : Word):
     0 <= idx' < SIZE_MAP ->
     idx ≠ idx' ->
-    isKVS b m ∗
+    isKVS b m s ∗
     k ⤇(KVS)[ idx ] w -∗
     ∃ k' w',
       ⌜ k ≠ k' ⌝ ∗ ⌜ m !! idx' = Some (k', w') ⌝ ∗
-      isKVS_open b m idx' ∗
+      isKVS_open b m s idx' ∗
       k ⤇(KVS)[ idx ] w ∗
       isKVS_entry b idx' (k', w').
   Proof.
-    iIntros (Hidx' Hidx_ne) "( (%Hwf & Hkvs_auth & HKVS) & Hk)".
+    iIntros (Hidx' Hidx_ne) "( (%Hwf_kvs & Hkvs_auth & Halloc & %Hwf_alloc & HKVS) & Hk)".
     iDestruct (kvs_valid with "Hkvs_auth Hk") as "%Hm_idx".
-    pose proof (wf_kvs_is_Some _ _ Hwf Hidx') as [ [k' w'] Hm_idx' ].
-    pose proof (wf_kvs_neq _ _ _ _ _ _ _ Hwf Hidx_ne Hm_idx Hm_idx') as Hkk'.
+    pose proof (wf_kvs_is_Some _ _ Hwf_kvs Hidx') as [ [k' w'] Hm_idx' ].
+    pose proof (wf_kvs_neq _ _ _ _ _ _ _ Hwf_kvs Hidx_ne Hm_idx Hm_idx') as Hkk'.
     iExists k',w'.
     rewrite -{2}(insert_id m idx' (k',w')); last done.
     iDestruct (big_sepM_insert_delete with "HKVS") as "[ [Hkb' Hkw'] HKVS]".
     iFrame; eauto.
   Qed.
 
-  Lemma close_isKVS
-    (b : Addr) (m : kvs_map) (idx : nat) (k : Z) (w : Word):
-    m !! idx = Some (k, w) ->
-    isKVS_open b m idx ∗
-    isKVS_entry b idx (k, w) -∗
-    isKVS b m.
+  Lemma open_isKVS_not_alloc
+    (b : Addr) (m : kvs_map) (s s' : gset (Z*Z))
+    (idx : nat) (ku kn : Z) :
+    let fkey := kvs_full_key ku kn in
+    (0 ≤ idx < SIZE_MAP)%Z →
+    (ku, kn) ∉ s' →
+    isKVS b m s -∗
+    ◯(ALLOC)[ku] s' -∗
+    ∃ kidx widx,
+      ⌜ kidx ≠ fkey ⌝ ∗
+      ⌜ m !! idx = Some (kidx, widx) ⌝ ∗
+      isKVS_open b m s idx ∗
+      ◯(ALLOC)[ku] s' ∗
+      isKVS_entry b idx (kidx, widx).
   Proof.
-    iIntros (Hidx) "[(%Hwf & Hkvs_auth & HKVS) Hkvs_entry]"; cbn.
+    intros fkey Hidx Hs'.
+    iIntros "(%Hwf_kvs & Hkvs_auth & Halloc & %Hwf_alloc & HKVS) Hk".
+    iDestruct ( allocated_keys_valid with "Halloc Hk" ) as "%Hss'".
+    assert (fkey ∉ kvs_keys m) as Hfkey_not_allocated.
+    { intro Hcontra; apply (Hwf_alloc (ku, kn)) in Hcontra.
+      rewrite /kvs_alloc_synced in Hwf_alloc.
+      set_solver. }
+    iFrame.
+    assert ( is_Some (m !! idx) ) as [ [kidx widx] Hm_idx].
+    { apply wf_kvs_is_Some; auto; lia. }
+    rewrite -{1}(insert_id m idx (kidx, widx)); last done.
+    iDestruct (big_sepM_insert_delete with "HKVS") as "[Hkvs_entry HKVS]".
+    iFrame "∗%".
+    iPureIntro.
+    assert ( kidx ∈ kvs_keys m ) as Hkidx by (apply elem_of_kvs_keys; eauto).
+    set_solver.
+  Qed.
+
+  Lemma open_isKVS
+    (b : Addr) (m : kvs_map) (s  : gset (Z*Z))
+    (idx : nat) :
+    (0 ≤ idx < SIZE_MAP)%Z →
+    isKVS b m s -∗
+    ∃ kidx widx,
+      ⌜ m !! idx = Some (kidx, widx) ⌝ ∗
+      isKVS_open b m s idx ∗
+      isKVS_entry b idx (kidx, widx).
+  Proof.
+    intros Hidx.
+    iIntros "(%Hwf_kvs & Hkvs_auth & Halloc & %Hwf_alloc & HKVS)".
+    iFrame.
+    assert ( is_Some (m !! idx) ) as [ [kidx widx] Hm_idx].
+    { apply wf_kvs_is_Some; auto; lia. }
+    rewrite -{1}(insert_id m idx (kidx, widx)); last done.
+    iDestruct (big_sepM_insert_delete with "HKVS") as "[Hkvs_entry HKVS]".
+    iFrame "∗%".
+  Qed.
+
+  Lemma close_isKVS
+    (b : Addr) (m : kvs_map) (s : gset (Z*Z)) (idx : nat) (k : Z) (w : Word):
+    m !! idx = Some (k, w) ->
+    isKVS_open b m s idx ∗
+    isKVS_entry b idx (k, w) -∗
+    isKVS b m s.
+  Proof.
+    iIntros (Hidx) "[(%Hwf_kvs & Hkvs_auth & Halloc & %Hwf_alloc & HKVS) Hkvs_entry]"; cbn.
     iDestruct (big_sepM_delete with "[$HKVS $Hkvs_entry]") as "HKVS"; eauto.
     iFrame; eauto.
   Qed.
 
-  Lemma isKVS_open_update (a : Addr) (m : kvs_map) (idx : nat) (k : Z) (w w' : Word) :
-    isKVS_open a m idx -∗ k ⤇(KVS)[ idx ] w
-    ==∗
-    isKVS_open a (<[idx:=(k, w')]> m) idx ∗ k ⤇(KVS)[ idx ] w'.
+  Lemma kvs_alloc_synced_update (m : kvs_map) ( s : gset (Z*Z) ) (idx : nat) (k : Z) (w : Word) :
+    (∃ w', m !! idx = Some (k, w')) ->
+    kvs_alloc_synced m s ->
+    kvs_alloc_synced (<[idx:=(k, w)]> m) s.
   Proof.
-    iIntros "(%Hkvs_wf & Hkvs_auth & HKVS) Hk".
+    intros [w' Hidx] Halloc.
+    rewrite /kvs_alloc_synced.
+    intros [ku kn].
+    specialize (Halloc (ku, kn)); cbn in *.
+    split; intros Hk.
+    - apply Halloc in Hk.
+      apply elem_of_kvs_keys in Hk as (idx' & v' & Hk).
+      destruct (decide (idx = idx')); simplify_eq; cbn in *.
+      + by eapply elem_of_kvs_keys; eexists idx',_; simplify_map_eq.
+      + by eapply elem_of_kvs_keys; eexists idx',_; simplify_map_eq.
+    - apply Halloc.
+      apply elem_of_kvs_keys in Hk as (idx' & v' & Hk).
+      destruct (decide (idx = idx')); simplify_eq; cbn in *.
+      + by eapply elem_of_kvs_keys; eexists idx',_; simplify_map_eq.
+      + by eapply elem_of_kvs_keys; eexists idx',_; simplify_map_eq.
+  Qed.
+
+  Lemma isKVS_open_update (a : Addr) (m : kvs_map) (s : gset (Z*Z)) (idx : nat) (k : Z) (w w' : Word) :
+    isKVS_open a m s idx -∗ k ⤇(KVS)[ idx ] w
+    ==∗
+    isKVS_open a (<[idx:=(k, w')]> m) s idx ∗ k ⤇(KVS)[ idx ] w'.
+  Proof.
+    iIntros "(%Hwf_kvs & Hkvs_auth & Halloc & %Hwf_alloc & HKVS) Hk".
     iDestruct (kvs_valid with "Hkvs_auth Hk") as "%Hm_idx".
     iMod (kvs_auth_update a m idx _ k _ w' with "Hkvs_auth Hk") as "[$ $]".
-    eapply (wf_kvs_map_insert _ _ _ w') in Hkvs_wf; eauto.
-    iModIntro.
-    iSplit; first by iPureIntro.
-    by rewrite delete_insert_eq.
+    eapply (wf_kvs_map_update _ _ _ w') in Hwf_kvs; eauto.
+    eapply (kvs_alloc_synced_update _ _ _ _ w') in Hwf_alloc; eauto.
+    rewrite delete_insert_eq.
+    by iFrame "∗ %".
+  Qed.
+
+  Lemma isKVS_open_insert (a : Addr) (m : kvs_map) (s s' : gset (Z*Z)) (idx : nat) (ku kn : Z) (w : Word) :
+    let k := kvs_full_key ku kn in
+    (ku, kn) ∉  s' →
+    isKVS_open a m s idx -∗
+    ◯(ALLOC)[ku] s' -∗
+    EMPTY_SLOT ⤇(KVS)[ idx ] (WInt DEFAULT_VAL)
+    ==∗
+    isKVS_open a (<[idx:=(k, w)]> m) ({[(ku, kn)]} ∪ s) idx ∗
+    ◯(ALLOC)[ku] ({[(ku, kn)]} ∪ s') ∗
+    k ⤇(KVS)[ idx ] w.
+  Proof.
+    intro k.
+    iIntros (Hs') "(%Hwf_kvs & Hkvs_auth & Halloc_auth & %Hwf_alloc & HKVS) Halloc_frag Hk".
+    iDestruct (allocated_keys_valid with "Halloc_auth Halloc_frag") as "->".
+    iDestruct (kvs_valid with "Hkvs_auth Hk") as "%Hm_idx".
+    iMod (kvs_auth_update a m idx _ k _ w with "Hkvs_auth Hk") as "[$ $]".
+    iMod ( allocated_keys_insert ku kn with "Halloc_auth Halloc_frag") as "[Halloc_auth Halloc_frag]".
+    rewrite /kvs_alloc_synced in Hwf_alloc.
+    assert (k ∉ kvs_keys m) as Hk_notin_keys.
+    { intro Hcontra; apply Hs'. apply elem_of_filter; cbn in *; split; auto.
+      apply Hwf_alloc; cbn; done. }
+    eapply (wf_kvs_map_insert _ _ _ w) in Hwf_kvs; eauto.
+    eapply (kvs_alloc_synced_insert _ _ _ _ _ w) in Hwf_alloc; eauto.
+    rewrite delete_insert_eq.
+    subst k.
+    by iFrame "∗ %".
   Qed.
 
   Lemma KVS_getFullKey_spec `{KVS : kvsLayout}
@@ -378,11 +620,11 @@ Section KVS_preamble.
     iApply "Hpost"; iFrame.
   Qed.
 
-  Lemma KVS_search_spec `{KVS : kvsLayout}
+  Lemma KVS_search_spec_in `{KVS : kvsLayout}
     (pc_b pc_e pc_a : Addr)
     (cgp_b cgp_e : Addr)
     (rkey ridx rscratch : RegName)
-    (m : kvs_map) (idx : nat) (fkey : Z) (w : Word)
+    (m : kvs_map) (s : gset (Z*Z)) (idx : nat) (fkey : Z) (w : Word)
     :
     let instrs := (kvs_search_instrs rkey ridx rscratch) in
     SubBounds pc_b pc_e pc_a (pc_a ^+ length instrs)%a ->
@@ -400,7 +642,7 @@ Section KVS_preamble.
       ridx ↦ᵣ - ∗
       rscratch ↦ᵣ - ∗
 
-      isKVS (cgp_b ^+ 1)%a m ∗
+      isKVS (cgp_b ^+ 1)%a m s ∗
       fkey ⤇(KVS)[idx] w ∗
 
       codefrag pc_a instrs ∗
@@ -411,10 +653,10 @@ Section KVS_preamble.
           ridx ↦ᵣ WInt idx ∗
           rscratch ↦ᵣ - ∗
 
-          isKVS_open (cgp_b ^+ 1)%a m (idx) ∗
+          isKVS_open (cgp_b ^+ 1)%a m s idx ∗
           (cgp_b ^+ (1+2*idx))%a ↦ₐ WInt fkey ∗
           (cgp_b ^+ (2+2*idx))%a ↦ₐ w ∗
-          isKVS_entry_empty idx fkey w ∗
+          isKVS_entry_empty idx fkey ∗
 
           ⌜ withinBounds cgp_b cgp_e (cgp_b ^+ (2 + 2 * idx))%a = true ⌝ ∗
 
@@ -486,7 +728,7 @@ Section KVS_preamble.
       iApply "Hpost"; iFrame.
       iPureIntro; rewrite /withinBounds; solve_addr.
 
-    - iDestruct (open_isKVS_kvs_frag_idx_diff _ _ _ (Z.to_nat n) with "[$HKVS $Hkvs_frag]")
+    - iDestruct (open_isKVS_kvs_frag_idx_diff _ _ _ _ (Z.to_nat n) with "[$HKVS $Hkvs_frag]")
         as "(%k' & %w' & %Hkk' & %Hm_idx' & HKVS  & Hkvs_frag & (Hbk & Hbw & Hfkey))".
       { lia. }
       { lia. }
@@ -522,6 +764,299 @@ Section KVS_preamble.
         intros idx' Hidx'_bound.
         destruct (decide (idx' = Z.to_nat n)%Z) as [-> | Hidx']; eauto.
         apply Hfkey_notin_nfirst; lia.
+  Qed.
+
+  Lemma KVS_search_spec_notin `{KVS : kvsLayout}
+    (pc_b pc_e pc_a : Addr)
+    (cgp_b cgp_e : Addr)
+    (rkey ridx rscratch : RegName)
+    (m : kvs_map) (s s' : gset (Z*Z)) (ku kn : Z)
+    :
+    let instrs := (kvs_search_instrs rkey ridx rscratch) in
+    let fkey := kvs_full_key ku kn in
+    SubBounds pc_b pc_e pc_a (pc_a ^+ length instrs)%a ->
+    withinBounds cgp_b cgp_e cgp_b = true ->
+    ((cgp_b + (1 + 2*SIZE_MAP)%Z)%a = Some cgp_e)%a ->
+    (ku, kn) ∉ s' ->
+
+    rscratch ≠ cnull ->
+    ridx ≠ cnull ->
+    rkey ≠ cnull ->
+
+    (
+      PC ↦ᵣ WCap RX Global pc_b pc_e pc_a ∗
+      cgp ↦ᵣ WCap RW Global cgp_b cgp_e (cgp_b ^+ 1 )%a ∗
+      rkey ↦ᵣ WInt fkey ∗
+      ridx ↦ᵣ - ∗
+      rscratch ↦ᵣ - ∗
+
+      isKVS (cgp_b ^+ 1)%a m s ∗
+      ◯(ALLOC)[ku] s' ∗
+
+      codefrag pc_a instrs ∗
+      ▷ (
+          PC ↦ᵣ WCap RX Global pc_b pc_e (pc_a ^+ length instrs)%a ∗
+          cgp ↦ᵣ WCap RW Global cgp_b cgp_e (cgp_b ^+ 1)%a ∗
+          rkey ↦ᵣ WInt fkey ∗
+          ridx ↦ᵣ WInt (-1) ∗
+          rscratch ↦ᵣ - ∗
+
+          isKVS (cgp_b ^+ 1)%a m s ∗
+          ◯(ALLOC)[ku] s' ∗
+
+          codefrag pc_a instrs -∗
+
+          WP Seq (Instr Executable) {{ v, ⌜v = HaltedV⌝ → na_own logrel_nais ⊤ }}
+        )
+      ⊢ WP Seq (Instr Executable) {{ v, ⌜v = HaltedV⌝ → na_own logrel_nais ⊤ }})%I.
+  Proof.
+    intros instrs fkey ; subst instrs.
+    iIntros (HsubBounds Hbounds_cgp Hcgp_bound Hs' Hrscratch Hridx Hkey)
+      "(HPC & Hcgp & Hrkey & [%wridx Hridx] & Hrscratch & HKVS & Halloc & Hcode & Hpost)".
+    codefrag_facts "Hcode"; rename H into Hpc_contiguous ; clear H0.
+
+    (* Mov ridx 0 *)
+    iInstr "Hcode".
+
+    remember 0%Z as n.
+    iAssert (⌜ (0 <= n <= SIZE_MAP)%Z ⌝)%I as "%Hn"; first (iPureIntro ; lia).
+    rewrite{1} (_ : (cgp_b ^+ 1)%a = (cgp_b ^+ (1 + 2 * n))%a); last by solve_addr.
+    assert (forall i, (0 <= i < Z.to_nat n) -> ∃ (k : Z) (w : Word),  m !! i = Some (k,w) ∧ k ≠ fkey)
+    as Hfkey_notin_nfirst.
+    { rewrite Heqn; intros i Hi; lia. }
+    clear Heqn.
+
+    iLöb as "IH" forall (n Hn Hfkey_notin_nfirst).
+
+    (* sub rscratch SIZE_MAP ridx; *)
+    iDestruct "Hrscratch" as "[%wrscratch Hrscratch]".
+    iInstr "Hcode".
+    replace 16 with SIZE_MAP by (by rewrite /SIZE_MAP).
+    destruct (decide ((SIZE_MAP - n) = 0)%Z) as [Hneq|Hneq].
+    { (* End of the loop. *)
+      rewrite Hneq.
+      assert ( n = SIZE_MAP ) as -> by lia.
+
+      (* jnz (".loop_body")%asm rscratch; *)
+      iInstr "Hcode".
+      (* jmp (".loop_end_not_found")%asm; *)
+      iInstr "Hcode".
+
+      (* lea cgp (-(2*SIZE_MAP))%Z; *)
+      iInstr "Hcode".
+      { transitivity (Some (cgp_b ^+ 1)%a); rewrite /SIZE_MAP in Hcgp_bound |- *; solve_addr. }
+      (* mov ridx (-1)%Z; *)
+      iInstr "Hcode".
+      rewrite decide_False //=.
+      iApply "Hpost"; iFrame.
+    }
+    assert (0 ≤ n < SIZE_MAP)%Z as Hn' by lia.
+    (* jnz (".loop_body")%asm rscratch; *)
+    iInstr "Hcode".
+    { by injection. }
+
+  iDestruct (open_isKVS_not_alloc _ _ _ _ (Z.to_nat n) with "HKVS Halloc")
+    as "(%kidx' & %widx & %Hkidx_ne & %Hm_kidx & HKVS & Halloc & (Hbk & Hbw & Hfkey))" ; eauto; [lia|].
+  replace ((cgp_b ^+ 1) ^+ 2 * Z.to_nat n)%a  with (cgp_b ^+ (1 + 2 * n))%a by solve_addr+Hn.
+  replace ((cgp_b ^+ 1) ^+ (2 * Z.to_nat n + 1))%a with (cgp_b ^+ (2 + 2 * n))%a by solve_addr+Hn.
+
+  (* load rscratch cgp; *)
+  iInstr "Hcode".
+  { split; [done | solve_addr]. }
+  (* sub rscratch rkey rscratch; *)
+  iInstr "Hcode".
+  (* jnz (".not_same_key")%asm rscratch; *)
+  iInstr "Hcode".
+  { injection; cbn; lia. }
+  (* lea cgp 2; *)
+  iInstr "Hcode".
+  { transitivity (Some ( (cgp_b ^+ (1 + 2 * (n+1)))%a)); solve_addr. }
+  (* add ridx ridx 1; *)
+  iInstr "Hcode".
+  (* jmp (".loop_start"); *)
+  iInstr "Hcode".
+  { transitivity (Some ( (pc_a ^+ 1)%a)); solve_addr. }
+
+  iDestruct (close_isKVS with "[$HKVS Hbk Hbw Hfkey]") as "HKVS";eauto.
+  {
+    replace (cgp_b ^+ (1 + 2 * n))%a with ((cgp_b ^+ 1) ^+ 2 * Z.to_nat n)%a by solve_addr+Hn.
+    replace (cgp_b ^+ (2 + 2 * n))%a  with ((cgp_b ^+ 1) ^+ (2 * Z.to_nat n + 1))%a by solve_addr+Hn.
+    iFrame.
+  }
+
+  iApply ("IH" with "[] [] [$Hcgp] [$Hrkey] [$Hrscratch] [$HKVS] [$Halloc] [$Hpost] [$Hcode] [$HPC] [$Hridx]").
+    + iPureIntro; lia.
+    + iPureIntro.
+      intros idx' Hidx'_bound.
+      destruct (decide (idx' = Z.to_nat n)%Z) as [-> | Hidx']; eauto.
+      apply Hfkey_notin_nfirst; lia.
+  Qed.
+
+  Lemma KVS_search_spec_empty_slot `{KVS : kvsLayout}
+    (pc_b pc_e pc_a : Addr)
+    (cgp_b cgp_e : Addr)
+    (rkey ridx rscratch : RegName)
+    (m : kvs_map) (s : gset (Z*Z))
+    :
+    let instrs := (kvs_search_instrs rkey ridx rscratch) in
+    SubBounds pc_b pc_e pc_a (pc_a ^+ length instrs)%a ->
+    withinBounds cgp_b cgp_e cgp_b = true ->
+    ((cgp_b + (1 + 2*SIZE_MAP)%Z)%a = Some cgp_e)%a ->
+
+    rscratch ≠ cnull ->
+    ridx ≠ cnull ->
+    rkey ≠ cnull ->
+
+    (
+      PC ↦ᵣ WCap RX Global pc_b pc_e pc_a ∗
+      cgp ↦ᵣ WCap RW Global cgp_b cgp_e (cgp_b ^+ 1 )%a ∗
+      rkey ↦ᵣ WInt EMPTY_SLOT ∗
+      ridx ↦ᵣ - ∗
+      rscratch ↦ᵣ - ∗
+
+      isKVS (cgp_b ^+ 1)%a m s ∗
+
+      codefrag pc_a instrs ∗
+      ▷ ( (* An empty slot was found*)
+          ( ∃ idx_empty_slot : nat,
+            (
+            PC ↦ᵣ WCap RX Global pc_b pc_e (pc_a ^+ length instrs)%a ∗
+            cgp ↦ᵣ WCap RW Global cgp_b cgp_e (cgp_b ^+ (1+2*idx_empty_slot))%a ∗
+            rkey ↦ᵣ WInt EMPTY_SLOT ∗
+            ridx ↦ᵣ WInt idx_empty_slot ∗
+            rscratch ↦ᵣ - ∗
+
+            isKVS_open (cgp_b ^+ 1)%a m s idx_empty_slot ∗
+            (cgp_b ^+ (1+2*idx_empty_slot))%a ↦ₐ WInt EMPTY_SLOT ∗
+            (cgp_b ^+ (2+2*idx_empty_slot))%a ↦ₐ WInt DEFAULT_VAL ∗
+            EMPTY_SLOT ⤇(KVS)[ idx_empty_slot ] WInt DEFAULT_VAL ∗
+
+            ⌜ withinBounds cgp_b cgp_e (cgp_b ^+ (2 + 2 * idx_empty_slot))%a = true ⌝ ∗
+            ⌜ 0 <= idx_empty_slot ⌝ ∗
+
+            codefrag pc_a instrs
+            )
+          )
+          ∨ (* No empty slot found*)
+            (
+              PC ↦ᵣ WCap RX Global pc_b pc_e (pc_a ^+ length instrs)%a ∗
+              cgp ↦ᵣ WCap RW Global cgp_b cgp_e (cgp_b ^+ 1)%a ∗
+              rkey ↦ᵣ WInt EMPTY_SLOT ∗
+              ridx ↦ᵣ WInt (-1) ∗
+              rscratch ↦ᵣ - ∗
+
+              isKVS (cgp_b ^+ 1)%a m s ∗
+
+              codefrag pc_a instrs
+            ) -∗
+          WP Seq (Instr Executable) {{ v, ⌜v = HaltedV⌝ → na_own logrel_nais ⊤ }}
+        )
+      ⊢ WP Seq (Instr Executable) {{ v, ⌜v = HaltedV⌝ → na_own logrel_nais ⊤ }})%I.
+  Proof.
+    intros instrs ; subst instrs.
+    iIntros (HsubBounds Hbounds_cgp Hcgp_bound Hrscratch Hridx Hkey)
+      "(HPC & Hcgp & Hrkey & [%wridx Hridx] & Hrscratch & HKVS & Hcode & Hpost)".
+    codefrag_facts "Hcode"; rename H into Hpc_contiguous ; clear H0.
+
+    (* Mov ridx 0 *)
+    iInstr "Hcode".
+
+    remember 0%Z as n.
+    iAssert (⌜ (0 <= n <= SIZE_MAP)%Z ⌝)%I as "%Hn"; first (iPureIntro ; lia).
+    rewrite{1} (_ : (cgp_b ^+ 1)%a = (cgp_b ^+ (1 + 2 * n))%a); last by solve_addr.
+    assert (forall i, (0 <= i < Z.to_nat n) -> ∃ (k : Z) (w : Word),  m !! i = Some (k,w) ∧ k ≠ EMPTY_SLOT)
+    as Hfkey_notin_nfirst.
+    { rewrite Heqn; intros i Hi; lia. }
+    clear Heqn.
+
+    iLöb as "IH" forall (n Hn Hfkey_notin_nfirst).
+
+    (* sub rscratch SIZE_MAP ridx; *)
+    iDestruct "Hrscratch" as "[%wrscratch Hrscratch]".
+    iInstr "Hcode".
+    replace 16 with SIZE_MAP by (by rewrite /SIZE_MAP).
+    destruct (decide ((SIZE_MAP - n) = 0)%Z) as [Hneq|Hneq].
+    { (* End of the loop. *)
+      rewrite Hneq.
+      assert ( n = SIZE_MAP ) as -> by lia.
+
+      (* jnz (".loop_body")%asm rscratch; *)
+      iInstr "Hcode".
+      (* jmp (".loop_end_not_found")%asm; *)
+      iInstr "Hcode".
+
+      (* lea cgp (-(2*SIZE_MAP))%Z; *)
+      iInstr "Hcode".
+      { transitivity (Some (cgp_b ^+ 1)%a); rewrite /SIZE_MAP in Hcgp_bound |- *; solve_addr. }
+      (* mov ridx (-1)%Z; *)
+      iInstr "Hcode".
+      rewrite decide_False //=.
+      iApply "Hpost"; iRight; iFrame.
+    }
+    assert (0 ≤ n < SIZE_MAP)%Z as Hn' by lia.
+    (* jnz (".loop_body")%asm rscratch; *)
+    iInstr "Hcode".
+    { by injection. }
+
+  iDestruct (open_isKVS _ _ _ (Z.to_nat n) with "HKVS") as "(%kidx' & %widx & %Hm_kidx & HKVS & (Hbk & Hbw & Hfkey))"
+  ; eauto; [lia|].
+  replace ((cgp_b ^+ 1) ^+ 2 * Z.to_nat n)%a  with (cgp_b ^+ (1 + 2 * n))%a by solve_addr+Hn.
+  replace ((cgp_b ^+ 1) ^+ (2 * Z.to_nat n + 1))%a with (cgp_b ^+ (2 + 2 * n))%a by solve_addr+Hn.
+  iEval (cbn) in "Hbk"; iEval (cbn) in "Hbw"; iEval (cbn) in "Hfkey".
+
+  (* load rscratch cgp; *)
+  iInstr "Hcode".
+  { split; [done | solve_addr]. }
+  (* sub rscratch rkey rscratch; *)
+  iInstr "Hcode".
+
+  rewrite /isKVS_entry_empty.
+  destruct (decide (kidx' = EMPTY_SLOT)) as [Hkidx'_empty |  Hkidx'_empty]; simplify_eq.
+  - (* Empty slot found *)
+    replace (Z.sub EMPTY_SLOT EMPTY_SLOT) with 0%Z by lia.
+    (* jnz (".not_same_key")%asm rscratch; *)
+    iInstr "Hcode".
+    (* jmp (".loop_end_found")%asm; *)
+    iInstr "Hcode".
+
+    iDestruct (isKVS_open_valid with "HKVS Hfkey") as "%Hm_kidx_eq"; simplify_map_eq.
+    replace (cgp_b ^+ (1 + 2 * n))%a with (cgp_b ^+ (1 + 2 * Z.to_nat n))%a by solve_addr+Hn.
+    replace (cgp_b ^+ (2 + 2 * n))%a  with (cgp_b ^+ (2 + 2 * Z.to_nat n))%a by solve_addr+Hn.
+
+
+    assert (((Z.of_nat (Z.to_nat n))) = n) as Hn_eq by lia.
+    rewrite -{1}Hn_eq.
+    iApply "Hpost"; iLeft; iFrame.
+    iPureIntro; rewrite /withinBounds; solve_addr.
+
+  - (* Empty slot not found *)
+
+    (* jnz (".not_same_key")%asm rscratch; *)
+    iInstr "Hcode".
+    { injection; cbn; lia. }
+    (* lea cgp 2; *)
+    iInstr "Hcode".
+    { transitivity (Some ( (cgp_b ^+ (1 + 2 * (n+1)))%a)); solve_addr. }
+    (* add ridx ridx 1; *)
+    iInstr "Hcode".
+    (* jmp (".loop_start"); *)
+    iInstr "Hcode".
+    { transitivity (Some ( (pc_a ^+ 1)%a)); solve_addr. }
+
+    iDestruct (close_isKVS with "[$HKVS Hbk Hbw Hfkey]") as "HKVS";eauto.
+    {
+      replace (cgp_b ^+ (1 + 2 * n))%a with ((cgp_b ^+ 1) ^+ 2 * Z.to_nat n)%a by solve_addr+Hn.
+      replace (cgp_b ^+ (2 + 2 * n))%a  with ((cgp_b ^+ 1) ^+ (2 * Z.to_nat n + 1))%a by solve_addr+Hn.
+      rewrite /isKVS_entry /isKVS_entry_empty /= decide_False //.
+      iFrame.
+    }
+
+    iApply ("IH" with "[] [] [$Hcgp] [$Hrkey] [$Hrscratch] [$HKVS] [$Hpost] [$Hcode] [$HPC] [$Hridx]").
+    + iPureIntro; lia.
+    + iPureIntro.
+      intros idx' Hidx'_bound.
+      destruct (decide (idx' = Z.to_nat n)%Z) as [-> | Hidx']; eauto.
+      apply Hfkey_notin_nfirst; lia.
   Qed.
 
 End KVS_preamble.
